kuiops/sdpa/Kuiops.Sdpa.Flash.fst
@@ -40,7 +40,7 @@ module Trade = Pulse.Lib.Trade
 inline_for_extraction noextract
 let sdpa_flash_kd
   (#et_ab #et_acc : Type0)
-  {| floating et_acc |} {| real_like et_acc |}
+  {| floating et_acc |} {| real_like et_acc |} {| floating_real_like et_acc |}
   {| scalar et_ab |} {| real_like et_ab |}
   {| FC.float_cast et_ab et_acc |}
   {| FC.float_cast et_acc et_ab |}
@@ -180,7 +180,7 @@ let sdpa_flash_kd
 inline_for_extraction noextract
 fn sdpa_flash_async
   (#et_ab #et_acc : Type0)
-  {| floating et_acc |} {| real_like et_acc |}
+  {| floating et_acc |} {| real_like et_acc |} {| floating_real_like et_acc |}
   {| scalar et_ab |} {| real_like et_ab |}
   {| FC.float_cast et_ab et_acc |}
   {| FC.float_cast et_acc et_ab |}
