kuiops/sdpa/Kuiops.Sdpa.Flash.fsti
@@ -19,7 +19,7 @@ module FC = Kuiper.Float.Casts
 inline_for_extraction noextract
 fn sdpa_flash_async
   (#et_ab #et_acc : Type0)
-  {| floating et_acc |} {| real_like et_acc |}
+  {| floating et_acc |} {| real_like et_acc |} {| floating_real_like et_acc |}
   {| scalar et_ab |} {| real_like et_ab |}
   {| FC.float_cast et_ab et_acc |}
   {| FC.float_cast et_acc et_ab |}
